pulse/src/checker/Pulse.Readback.fst
@@ -18,14 +18,12 @@ module Pulse.Readback
 module R = FStar.Reflection.V2
 open Pulse.Syntax.Base
 open Pulse.Reflection.Util
+open Pulse.Common
 module RU = Pulse.RuntimeUtils
+module RT = FStar.Reflection.Typing
 module T = FStar.Tactics.V2
+module L = FStar.List.Tot.Base
 let debug_log (f: unit -> T.Tac unit) : T.Tac unit = if RU.debug_at_level_no_module "readback" then f()
-
-let (let?) (f:option 'a) (g:'a -> option 'b) : option 'b =
-  match f with
-  | None -> None
-  | Some x -> g x
 
 let readback_observability (t:R.term)
 : option (obs:observability { elab_observability obs == t })
@@ -124,3 +122,85 @@ let readback_comp (t:R.term)
   | _ ->
     let t' = t in
     Some (C_Tot t' <: c:comp{ elab_comp c == t })
+
+let rec readback_pat (p : R.pattern) : option pattern =
+  match p with
+  | R.Pat_Cons fv _ args ->
+    let fv = R.inspect_fv fv in
+    let? args = map_opt_dec p readback_sub_pat args in
+    Some (Pat_Cons {fv_name=fv; fv_range=Range.range_0} args)
+  | R.Pat_Constant c ->
+    Some (Pat_Constant c)
+  | R.Pat_Var st nm ->
+    Some (Pat_Var nm (RU.map_seal st RU.deep_compress))
+  | R.Pat_Dot_Term None -> Some (Pat_Dot_Term None)
+  | R.Pat_Dot_Term (Some t) ->
+    if R.Tv_Unknown? (R.inspect_ln t)
+    then None
+    else
+      let t = RU.deep_compress t in
+      let t = RU.set_range t Range.range_0 in
+      Some (Pat_Dot_Term (Some t))
+  | _ -> None
+and readback_sub_pat (pb : R.pattern & bool) : option (pattern & bool) =
+  let (p, b) = pb in
+  let? p = readback_pat p in
+  Some (p, b)
+
+#push-options "--fuel 2 --ifuel 2 --z3rlimit_factor 2"
+#restart-solver
+let rec elab_readback_pat_x (rp : R.pattern) (p : pattern)
+  : Lemma (requires readback_pat rp == Some p)
+          (ensures elab_pat p == rp)
+  = match rp, p with
+  | R.Pat_Cons r_fv r_us_opt r_subpats, Pat_Cons {fv_name=fv_name} subpats ->
+    assert (fv_name == R.inspect_fv r_fv);
+    assert (Some? (readback_pat rp));
+    let fv = R.inspect_fv r_fv in
+
+    assert (readback_pat rp ==
+             (let? args = map_opt_dec rp readback_sub_pat r_subpats in
+              Some (Pat_Cons {fv_name=fv; fv_range=Range.range_0} args)))
+        by (T.norm [delta; zeta]);
+
+    let aux1 (i:nat{i < L.length r_subpats})
+    : Lemma (r_subpats `L.index` i == (map_dec p subpats elab_sub_pat) `L.index` i)
+    =
+      lemma_map_opt_dec_index rp readback_sub_pat r_subpats subpats;
+      calc (==) {
+        map_dec p subpats elab_sub_pat `L.index` i;
+        == { lemma_map_dec_index_i p elab_sub_pat subpats i }
+        elab_sub_pat (subpats `L.index` i);
+        == { () }
+        elab_sub_pat (Some?.v (readback_sub_pat (r_subpats `L.index` i)));
+        == { elab_readback_subpat (r_subpats `L.index` i) }
+        r_subpats `L.index` i;
+      }
+    in
+    Classical.forall_intro aux1;
+    FStar.List.Tot.Properties.index_extensionality
+        (map_dec p subpats elab_sub_pat)
+        r_subpats;
+
+    assert (elab_pat p ==
+             R.Pat_Cons (R.pack_fv fv_name) None (map_dec p subpats elab_sub_pat))
+        by (T.norm [delta; zeta]);
+
+    assert (R.pack_fv fv_name == r_fv);
+    // FIXME: readback will drop the universe annotation, so we cannot
+    // really prove this. Should we add it to pulse pattern syntax?
+    assume (r_us_opt == None);
+    assert (r_subpats == map_dec p subpats elab_sub_pat);
+    ()
+
+  | R.Pat_Constant _, Pat_Constant _ -> ()
+  | R.Pat_Var st nm, Pat_Var _ _ ->
+    Sealed.sealed_singl st (Sealed.seal RT.tun);
+    ()
+  | _ -> ()
+and elab_readback_subpat (pb : R.pattern & bool)
+  : Lemma (requires (Some? (readback_sub_pat pb)))
+          (ensures elab_sub_pat (Some?.v (readback_sub_pat pb)) == pb)
+  = let (p, b) = pb in
+    elab_readback_pat_x p (Some?.v (readback_pat p))
+#pop-options
